src/core/DY.Core.Trace.State.Aux.fst
@@ -1,0 +1,137 @@
+module DY.Core.Trace.State.Aux
+
+open DY.Core.Trace.Type
+open DY.Core.Bytes.Type
+open DY.Core.Bytes
+open DY.Core.Label.Type
+
+type state_raw = bytes
+type session_raw = rev_list state_raw
+type full_state_raw = list (state_id * session_raw) 
+//TODO: this should be `Map state_id session_raw`, can we extract the generic Map part from DY.Lib.State.Map?
+// or is it not worth the effort?
+
+val max: int -> int -> int
+let max x y =
+  if x < y then y else x
+
+/// To add a new session to a state of a principal,
+/// we have to find a new identifier
+/// that is not used in the current state of the principal.
+
+val compute_new_session_id: principal -> trace -> state_id
+let rec compute_new_session_id prin tr =
+  match tr with
+  | Nil -> {the_id = 0}
+  | Snoc tr_init evt -> (
+    match evt with
+    | SetState prin' sess_id _ ->
+      if prin = prin' then
+        {the_id = 
+             max (sess_id.the_id + 1) (compute_new_session_id prin tr_init).the_id}
+      else
+        compute_new_session_id prin tr_init
+    | _ -> compute_new_session_id prin tr_init
+  )
+
+// Sanity check
+val compute_new_session_id_correct:
+  prin:principal -> tr:trace ->
+  sess_id:state_id -> state_content:bytes ->
+  Lemma
+  (requires event_exists tr (SetState prin sess_id state_content))
+  (ensures sess_id.the_id < (compute_new_session_id prin tr).the_id)
+let rec compute_new_session_id_correct prin tr sess_id state_content =
+  match tr with
+  | Nil -> ()
+  | Snoc tr_init evt -> (
+    if evt = SetState prin sess_id state_content then ()
+    else (
+      compute_new_session_id_correct prin tr_init sess_id state_content
+    )
+  )
+
+val get_state_aux: principal -> state_id -> trace -> option state_raw
+let rec get_state_aux prin sess_id tr =
+  match tr with
+  | Nil -> None
+  | Snoc tr_init (SetState prin' sess_id' content) -> (
+    if prin = prin' && sess_id = sess_id' then
+      Some content
+    else
+      get_state_aux prin sess_id tr_init
+  )
+  | Snoc tr_init _ ->
+      get_state_aux prin sess_id tr_init
+
+val get_session_aux: principal -> state_id -> trace -> session_raw
+let rec get_session_aux prin sess_id tr = 
+  match tr with
+  | Nil -> Nil
+  | Snoc init (SetState p' sid' content) ->
+      if p' = prin && sid' = sess_id
+        then Snoc (get_session_aux prin sess_id init) content
+        else (get_session_aux prin sess_id init)
+  | Snoc init _ -> (get_session_aux prin sess_id init)
+
+val get_session: principal -> state_id -> trace -> option session_raw
+let get_session prin sess_id tr =
+  match get_session_aux prin sess_id tr with
+  | Nil -> None
+  | sess -> Some sess
+  
+let _ =
+  let p = "a" in
+  let sid = {the_id = 1} in
+  let b = Literal (FStar.Seq.Base.empty) in
+  let tr = Snoc (Snoc Nil (SetState p sid b)) (SetState p sid b) in
+  assert(get_session p sid tr = Some (Snoc (Snoc Nil b) b));
+  assert(None? (get_session "b" sid tr))
+
+val append_to: #a:eqtype -> #b:Type -> list (a * rev_list b) -> a -> b -> list (a * rev_list b)
+let append_to xys key elem =
+  let (key_elems,rest) = FStar.List.Tot.Base.partition (fun (x, _) -> x = key) xys in
+  let new_key_elems = 
+    match key_elems with
+    | [] -> Snoc Nil elem
+    | Cons (k,elems) _ -> Snoc elems elem
+    in
+  (key, new_key_elems) :: rest // re-ordering shouldn't matter, since key is included
+
+let _ = 
+  let xs = [(1, Snoc Nil 5); (5, Nil)] in
+  assert(append_to xs 5 7 = [(5, Snoc Nil 7); (1, Snoc Nil 5)])
+
+val get_full_state_aux: principal -> trace -> full_state_raw -> full_state_raw
+let rec get_full_state_aux prin tr curr_state =
+  match tr with
+  | Nil -> curr_state
+  | Snoc init (SetState p' sid' content) ->
+      if p' = prin 
+        then begin
+          let new_state = append_to curr_state sid' content in
+          get_full_state_aux prin init new_state
+        end
+        else get_full_state_aux prin init curr_state
+  | Snoc init _ -> get_full_state_aux prin init curr_state
+
+val get_full_state: principal -> trace -> option full_state_raw
+let get_full_state prin tr = 
+  let next_state_id = compute_new_session_id prin tr in
+  if next_state_id.the_id = 0
+    then None
+    else begin
+      let full_state_init = [] in
+      match get_full_state_aux prin tr full_state_init with
+      | [] -> None
+      | fst -> Some fst
+    end
+
+let _ =
+  let p = "a" in
+  let sid1 = {the_id = 1} in
+  let sid2 = {the_id = 2} in
+  let b = Literal (FStar.Seq.Base.empty) in
+  let tr = Snoc (Snoc Nil (SetState p sid1 b)) (SetState p sid2 b) in
+  assert(get_full_state p tr = Some [(sid1, (Snoc Nil b)); (sid2, Snoc Nil b)]);
+  assert(None? (get_full_state "b" tr))
